theories/reflect/progdef.v
@@ -1,0 +1,36 @@
+(*
+ * Copyright (c) Meta Platforms, Inc. and affiliates.
+ *
+ * This source code is licensed under the MIT license found in the
+ * LICENSE file in the root directory of this source tree.
+ *)
+From stdpp Require Import base strings gmap stringmap fin_maps.
+(* Not using iris but importing their ssreflect dependencies *)
+From iris.proofmode Require Import tactics.
+From shack Require Import lang progdef.
+
+Section Reflect.
+  (* assume a given set of class definitions *)
+  Context `{PDC: ProgDefContext}.
+
+  Definition extendsb A B : bool :=
+    if pdefs !! A is Some adef then
+    if adef.(superclass) is Some (t, _) then String.eqb B t else false
+    else false
+  .
+
+  Lemma extendsb_correct A B : extendsb A B ↔ extends A B.
+  Proof.
+    rewrite /extendsb; split.
+    - destruct (pdefs !! A) as [adef | ] eqn:hadef; last done.
+      destruct (adef.(superclass)) as [(t, ?) | ] eqn:hsuper; last done.
+      move => heq.
+      destruct (B =? t) eqn:h; last done.
+      apply String.eqb_eq in h; subst.
+      by econstructor.
+    - move => h; destruct h as [A B adef σ hadef hsuper].
+      rewrite hadef hsuper.
+      destruct (B =? B) eqn:h; first done.
+      by rewrite eqb_neq in h.
+  Qed.
+End Reflect.
