theories/reflect/tactics.v
@@ -1,0 +1,46 @@
+(*
+ * Copyright (c) Meta Platforms, Inc. and affiliates.
+ *
+ * This source code is licensed under the MIT license found in the
+ * LICENSE file in the root directory of this source tree.
+ *)
+From stdpp Require Import base strings gmap stringmap fin_maps.
+(* Not using iris but importing their ssreflect dependencies *)
+From iris.proofmode Require Import tactics.
+
+From shack Require Import reflect.progdef.
+
+(* Helper tactics to deal with the `Acc` goal in progdef.v *)
+Lemma string_eqb_correct (s t: string) : (s =? t)%string ↔ s = t.
+Proof.
+  destruct String.eqb eqn:h.
+  - by apply String.eqb_eq in h as ->.
+  - apply String.eqb_neq in h.
+    by split.
+Qed.
+
+(* Do one step of Accessibility *)
+Ltac simpl_acc0 :=
+  constructor => ? /extendsb_correct;
+  rewrite /extendsb /=;
+  simpl_map => /=.
+
+(* If the previous tactic didn't solve the goal,
+ * rewrite.
+ *)
+Ltac simpl_acc1 := move/string_eqb_correct => ->.
+
+(* Gluing both tactics into an automated one *)
+Ltac simpl_acc_match :=
+  match goal with
+  | |- False → _ => done
+  | |- _ => (simpl_acc1; simpl_acc0)
+  end.
+
+Ltac simpl_acc := simpl_acc0; repeat simpl_acc_match.
+
+Ltac step_pacc :=
+  match goal with
+  | |- None = Some ?t → _ => done
+  | H : nat |- _ => destruct H; first (case => <-; simpl_acc)
+  end.
